### show me the derivation of e=mc^2

The equation e=mc^2, where e is the energy, m is the mass, and c is the speed of light, can be derived from the fundamental equation of special relativity, which is:

E^2 = (mc^2)^2 + (pc)^2

where p is the momentum.

To derive the equation e=mc^2, we can rearrange the above equation to isolate the energy term:

E^2 - (mc^2)^2 = (pc)^2

Then, we can take the square root of both sides to obtain:

|E| = sqrt((mc^2)^2 + (pc)^2)

Now, we can consider two cases:

If the particle is at rest (p=0), then we have:
|E| = sqrt((mc^2)^2 + (0)^2)

|E| = sqrt((mc^2)^2)

|E| = |mc^2|

Since the energy must be positive, we can simplify the equation to:

E = mc^2

If the particle is moving (p!=0), then we have:
|E| = sqrt((mc^2)^2 + (pc)^2)

In this case, the energy is not equal to the mass times the speed of light squared, but it is always greater than or equal to it, since the square root of a sum of squares is always greater than or equal to the square root of each individual square.

Therefore, the equation e=mc^2 is a special case of the more general equation for the energy of a particle in special relativity, and it holds only when the particle is at rest.